core/Extraction.v
@@ -2,11 +2,10 @@ Require Import ExtrOcamlZInt.
 Require Import ExtrOcamlString.
 Require Import ExtrOcamlBasic.
 
-(* Don't extract _rec(t) definitions *)
-Unset Elimination Schemes.
-
 Require Import Packet.
 Require Import Server.
+Require Import Serialize.
 
 Extraction Library Packet.
 Extraction Library Server.
+Extraction Library Serialize.
