core/Serialize.v
@@ -1,0 +1,128 @@
+Require Import ZArith.
+Require Import NArith.
+Require Import Coq.Strings.String.
+Require Import Ascii.
+
+Require Import Packet.
+
+Local Open Scope char_scope.
+Definition parse_opcode (data : string) : option (opcode * string) :=
+    match data with
+        | EmptyString => None
+        | String zero (String op tail) =>
+            match op with
+                | "001" => Some(RRQ, tail)
+                | "002" => Some(WRQ, tail)
+                | "003" => Some(DATA, tail)
+                | "004" => Some(ACK, tail)
+                | "005" => Some(ERROR, tail)
+                | _ => None
+            end
+        | _ => None
+    end.
+
+Lemma parsed_op_correct_value: forall (op : opcode) (tail : string),
+        parse_opcode (String zero (String
+            (ascii_of_pos (opcode_value (op)))
+            tail
+        )) = Some(op, tail).
+Proof.
+    intros.
+    destruct op.
+    all: simpl; reflexivity.
+Qed.
+
+Definition parse_errcode (data : string) : option (errcode * string) :=
+match data with
+    | EmptyString => None
+    | String zero (String op tail) =>
+        match op with
+            | "000" => Some(Undefined, tail)
+            | "001" => Some(FileNotFound, tail)
+            | "002" => Some(AccessViolation, tail)
+            | "003" => Some(AllocError, tail)
+            | "004" => Some(IllegalOp, tail)
+            | "005" => Some(UnknownTID, tail)
+            | "006" => Some(AlreadyExists, tail)
+            | "007" => Some(NoSuchUser, tail)
+            | _ => None
+        end
+    | _ => None
+end.
+
+Lemma parsed_err_correct_value: forall (err : errcode) (tail : string),
+        parse_errcode (String zero (String
+            (ascii_of_N (errcode_value (err)))
+            tail
+        )) = Some(err, tail).
+Proof.
+    intros.
+    destruct err.
+    all: simpl; reflexivity.
+Qed.
+
+(*
+TFTP Formats
+   Type   Op #     Format without header
+
+          2 bytes    string   1 byte     string   1 byte
+          -----------------------------------------------
+   RRQ/  | 01/02 |  Filename  |   0  |    Mode    |   0  |
+   WRQ    -----------------------------------------------
+          2 bytes    2 bytes       n bytes
+          ---------------------------------
+   DATA  | 03    |   Block #  |    Data    |
+          ---------------------------------
+          2 bytes    2 bytes
+          -------------------
+   ACK   | 04    |   Block #  |
+          --------------------
+          2 bytes  2 bytes        string    1 byte
+          ----------------------------------------
+   ERROR | 05    |  ErrorCode |   ErrMsg   |   0  |
+          ----------------------------------------
+*)
+
+(* ! Wykomentowane przez problemy z ekstrakcja *)
+Definition parse_data (data: string) : option packet :=
+    None.
+    (* match data with
+    | String c1 (String c2 tail) =>
+        let num := (nat_of_ascii(c1) * 256) + nat_of_ascii(c2) in
+            (* TODO: Handle mode: netascii replaces newline *)
+            match (length tail) <= 512 with
+            | True => Some(Data (N.of_nat num) tail)
+            end
+    | _ => None
+    end. *)
+
+Definition parse_error (data : string) : option packet :=
+    None.
+    (* match parse_errcode data with
+    | Some(errcode, String c tail) =>
+        let len := length (String c tail) in
+        match get len (String c tail) with
+        (* ErrMsg ends with 0 *)
+        | Some("000") =>
+            let errmsg := substring 0 (len-1) (String c tail) in
+                Some(Error errcode errmsg)
+        | _ => None
+        end
+    | _ => None
+    end. *)
+
+Definition parse_packet (data : string) : option packet :=
+    None.
+    (* match parse_opcode (data) with
+    | Some(RRQ, tail) => None (* TODO *)
+    | Some(WRQ, tail) => None (* TODO *)
+    | Some(DATA, tail) => parse_data tail
+    | Some(ACK, String c1 (String c2 EmptyString)) =>
+        let num := (nat_of_ascii(c1) * 256) + nat_of_ascii(c2) in
+            Some(Acknowledgment (N.of_nat num))
+    | Some(ERROR, tail) => parse_error tail
+    | _ => None
+    end. *)
+
+(* TODO *)
+Definition string_of_packet (p : packet) : string := EmptyString.
